\documentclass{article}
\usepackage{fancyhdr}
\usepackage{amsmath,amssymb}
\usepackage{geometry}
\usepackage{datetime}
\usepackage{enumerate}
\usepackage{graphicx}

%Insert page formatting here
\hoffset = -.5in
\voffset = -0.375in
\textwidth = 7in
\textheight = 8in
\headheight = 24pt

\pagestyle{fancy}

\rhead{Peter Olson\\Student ID: $441666$}
\lhead{Math 3200\\Homework 9}
\chead{\today}
\cfoot{}

%\addtolength{\headwidth}{\marginparsep}
%\addtolength{\headwidth}{\marginparwidth}

%\renewcommand{\labelitemi}{$\diamond$}
\renewcommand{\implies}{\rightarrow}
\newcommand{\widespace}{\qquad \qquad \;}
\newcommand{\tret}{\\ \hline}
\newcommand{\fh}{\tfrac{1}{2}}
\newcommand{\deriv}[2]{\frac{d #1}{d #2}}
\newcommand{\pderiv}[2]{\frac{\delta #1}{\delta #2}}
\newcommand{\vr}{\vec{r}}
\newcommand{\at}{\text{ at }}
\newcommand{\var}{\text{Var}}
\newcommand{\cov}{\text{Cov}}

\begin{document}

\section*{Exercise 10.14}

Show that $\bar{Y}$ and $\hat{\beta}_1$ are independent.

\begin{align*}
	\hat{Y} &= \tfrac{1}{n} \sum Y_i\\
	\hat{\beta}_1 &= \sum c_i Y_i \\
	c_i &= (x_i - \bar{x}) / S_{xx} \\
	\sum c_i &= 0 \\
	\cov(\bar{Y},\hat{\beta}_1) &= \sum \sum a_i b_j \cov (\bar{Y}_i,\hat{\beta}_{1i}) \\
	\cov (\bar{Y}_i,\hat{\beta}_{1i}) &= E[(\bar{Y}_i - \mu_{\bar{Y}_i})(\hat{\beta}_{1i} - \mu_{\hat{\beta}_{1i}})] \\
	&= E[(Y_i - Y)(c_iY_i - c_iY_i (\tfrac{1}{n}))] \\
	&= E[(Y_i - Y)(c_iY_i - c_iY)] \\
	&= c_i\cdot E[(Y_i - Y)^2] \\
	&= c_i\cdot \var(Y) \\
	\cov(\bar{Y},\hat{\beta}_1) &= \sum \sum a_i b_j c_i \cdot \var(Y) \\
	&= \sum 0 \cdot \sum a_i b_j \cdot \var(Y) \\
	\cov(\bar{Y},\hat{\beta}_1) &= 0 \\
\end{align*}

Because $\bar{Y}$ and $\hat{\beta}_1$ are uncorrelated, they then must be independent.


\section*{Exercise 10.33}

\[ \text{Show that   } \sum (y_i - \hat{y}_i)(\hat{y}_i - \bar{y}) = 0 \]

\begin{align*}
	\hat{y}_i &= \hat{\beta}_0 + \hat{\beta}_1x_i\\
	&= \bar{y} + \hat{\beta}_1(x_i - \bar{x})\\
	\sum (y_i - \hat{y}_i)(\hat{y}_i - \bar{y}) &= \sum (y_i - (\hat{\beta}_0 + \hat{\beta}_1x_i))((\hat{\beta}_0 + \hat{\beta}_1x_i) - (\hat{\beta}_0 + \hat{\beta}_1x_i - \hat{\beta}_0 + \hat{\beta}_1x_i)) \\
	&= \sum (y_i - (\hat{\beta}_0 + \hat{\beta}_1x_i))(- (\hat{\beta}_0 + \hat{\beta}_1x_i)) \\
	&= \sum y_i(- (\hat{\beta}_0 + \hat{\beta}_1x_i)) + \sum (\hat{\beta}_0 + \hat{\beta}_1x_i)^2 \\
	&=  \sum(- (\hat{\beta}_0 + \hat{\beta}_1x_i)) + \sum (\hat{\beta}_0 + \hat{\beta}_1x_i)^2 \\
	&= \sum y_i \hat{y}_i - \sum (\hat{y}_i)^2 \\
	\sum (y_i - \hat{y}_i)(\hat{y}_i - \bar{y}) &= 0
\end{align*}

\end{document}