\documentclass{article}
\usepackage{fancyhdr}
\usepackage{amsmath,amssymb}
\usepackage{geometry}
\usepackage{datetime}
\usepackage{enumerate}
\usepackage{graphicx}

%Insert page formatting here
%\hoffset = -.5in
\voffset = -0.375in
%\textwidth = 6in
\textheight = 8in
\headheight = 24pt

\pagestyle{fancy}

\rhead{Peter Olson\\Student ID: $441666$}
\lhead{Math 3200\\Homework 4}
\chead{\today}
\cfoot{}

%\addtolength{\headwidth}{\marginparsep}
%\addtolength{\headwidth}{\marginparwidth}

%\renewcommand{\labelitemi}{$\diamond$}
\renewcommand{\implies}{\rightarrow}
\newcommand{\widespace}{\qquad \qquad \;}
\newcommand{\tret}{\\ \hline}
\newcommand{\fh}{\tfrac{1}{2}}
\newcommand{\deriv}[2]{\frac{d #1}{d #2}}
\newcommand{\pderiv}[2]{\frac{\delta #1}{\delta #2}}
\newcommand{\vr}{\vec{r}}
\newcommand{\at}{\text{ at }}
\newcommand{\var}{\text{Var}}

\begin{document}
\section*{Exercise 2.43}
	For a random variable $X$ and constants $a$ and $b$, show that
	\[ \var(aX + b) = a^2 \var(X) \]
	
	\begin{align*}
		\text{Let } Y &= aX+b\\
		E(Y) &= aE(X) + b\\
		\var(Y) &= E\left[ Y - E(Y) \right]^2\\
		&= E \left[ aX + b - aE(X) - b \right]^2\\
		&= E \left[ aX - aE(X) \right]^2\\
		&= \left( aE \left[ X - E(X) \right] \right) ^2 \\
		\var(aX+b) &= a^2 E(X)^2\\
		\var(aX+b) &= a^2 \var(X)\\
	\end{align*}
\end{document}